test/bindings/Libsodium.fsti
@@ -1,0 +1,85 @@
+module Libsodium
+
+open FStar.Buffer
+open FStar.UInt8
+open Hacl.Constants
+
+(* For test purpose only (no specification associated) *)
+
+val crypto_box_beforenm:
+  k:uint8_p ->
+  pk:uint8_p ->
+  sk:uint8_p ->
+  Stack u32
+    (requires (fun _ -> True))
+    (ensures  (fun _ _ _ -> True))
+
+val crypto_box_detached:
+  c:uint8_p ->
+  mac:uint8_p ->
+  m:uint8_p ->
+  mlen:u64 ->
+  n:uint8_p ->
+  pk:uint8_p ->
+  sk:uint8_p ->
+  Stack u32
+    (requires (fun _ -> True))
+    (ensures  (fun _ _ _ -> True))
+
+val crypto_box_open_detached:
+  m:uint8_p ->
+  c:uint8_p ->
+  mac:uint8_p ->
+  mlen:u64 ->
+  n:uint8_p ->
+  pk:uint8_p ->
+  sk:uint8_p ->
+  Stack u32
+    (requires (fun _ -> True))
+    (ensures  (fun _ _ _ -> True))
+
+val crypto_box_easy:
+  c:uint8_p ->
+  m:uint8_p ->
+  mlen:u64 ->
+  n:uint8_p ->
+  pk:uint8_p ->
+  sk:uint8_p ->
+  Stack u32
+    (requires (fun _ -> True))
+    (ensures  (fun _ _ _ -> True))
+
+val crypto_box_open_easy:
+  m:uint8_p ->
+  c:uint8_p ->
+  mlen:u64 ->
+  n:uint8_p ->
+  pk:uint8_p ->
+  sk:uint8_p ->
+  Stack u32
+    (requires (fun _ -> True))
+    (ensures  (fun _ _ _ -> True))
+
+val crypto_box_keypair:
+  pk:uint8_p ->
+  sk:uint8_p ->
+  Stack unit
+    (requires (fun _ -> True))
+    (ensures  (fun _ _ _ -> True))
+
+val crypto_box_easy_afternm:
+  c:uint8_p ->
+  m:uint8_p ->
+  mlen:u64 ->
+  n:uint8_p ->
+  k:uint8_p ->
+  Stack unit
+    (requires (fun _ -> True))
+    (ensures  (fun _ _ _ -> True))
+
+val randombytes_buf:
+  b:uint8_p ->
+  blen:u64 ->
+  Stack unit
+    (requires (fun _ -> True))
+    (ensures  (fun _ _ _ -> True))
